$$
% \global\newcommand{\n}{\\ \ \\}
% \global\newcommand{\embrace}[3]{
%     \left#2
%         \begin{split}
%             #1
%         \end{split}
%     \right#3
% }
% \global\newcommand{\aembrace}[1]{
%     \embrace{#1}{\{}{\}}
% }
% \global\newcommand{\pembrace}[1]{
%     \embrace{#1}{(}{)}
% }
% \global\newcommand{\cembrace}[1]{
%     \embrace{#1}{[}{]}
% }
% \global\newcommand{\vec}[1]{\overrightarrow{#1}}
$$
# Ex 5
### <u>Théorème de Green</u>
$$
\iint_S \pembrace{\frac{\delta P}{\delta y}-\frac{\delta G}{\delta x}}dxdy=\oint_C \underbrace{P(x,y)dx+G(x,y)dy}_{\text{forme différentielle}}\n\n
\begin{split}
    \frac{\delta P}{\delta y} - \frac{\delta G}{\delta y}=1 \Rightarrow \underbrace{\iint_D dxdy}_{\text{Aide(D)}}&=\frac12\int-y\ dx+x\ dy\n
    &=\frac12\int x\ dy-y\ dx
\end{split}
$$

## Exercice d'application
$$
\text{<schema 4>}\n

\pembrace{\frac{x}{a}}^2+\pembrace{\frac{y}{b}}^2=1\n

A = \iint_D\ dxdy\n=\iint|det\ J|drd\theta\n

\embrace{&x=arcos\theta\\&y=brsin\theta}{\{}{.}\n

\embrace{&\frac{\delta x}{\delta r}\frac{ \delta x}{\delta \theta}\\&\frac{\delta y}{\delta r}\frac{\delta y}{\delta \theta}}{|}{|}=\embrace{&acos\theta\ \ -arsin\theta\\&bsin\theta\ \ \phantom{-}brcos\theta}{|}{|}\n

det|J_c|=abr\n\n\n

A = \int_0^1\int_0^{2\pi}abr\ d\theta\n
= 2rab\int_0^1rdr\
=2\pi ab\cembrace{\frac{r^2}{2}}_0^1\n
=\pi ab\n\n\n


\text{Autre méthode :}\n
A = \frac12 \int_C x\ dy-y\ dx\n

\embrace{&x=acos\theta\\&y=bsin\theta}{\{}{.}\Rightarrow \embrace{&dx=-asin\theta d\theta\\&dy=bcos\theta d\theta}{\{}{.}\n

A = \frac12 \int_0^{2\pi}acos\theta*bcos\theta d\theta - bsin\theta\pembrace{-asin\theta d\theta}\n
=\frac12\int_0^{2\pi}abcos^2\theta+ab\ sin^2\theta\ d\theta\n
=\frac12 \int_0^{2\pi}ab\ d\theta = \pi ab
$$

b) Soit d le domaine limité par les droites θ = θ1 et θ = θ2 et par la courbe d'équation polaire r = f(θ).
montrer que: 
$$
\text{aire(D)} = \iint_D dxdy = \frac12 \int_{\theta_1}^{\theta_2}\cembrace{f(\theta)}^2d\theta\n

\text{<schema 5>}\n

\text{aire(D)}=\frac12 \int x\ dy-y\ dx\n

\embrace{&x=f(\theta)cos\theta\\&y=f\theta)sin\theta}{\{}{.}\Rightarrow \embrace{&dx=-f'(x)sin\theta d\theta\\&dy=\phantom{-}f'(\theta)cos\theta d\theta}{\{}{.}\n

A=\frac12\int_{\Gamma_2^+}xdy-ydx\n

\embrace{&x=acos\theta\\&y=bsin\theta}{\{}{.}\Rightarrow \embrace{&dx=-asin\theta d\theta\\&dy=bcos\theta d\theta}{\{}{.}\n

A=\frac12\int f(\theta)cos\theta f'(\theta)cos\theta d\theta -f(\theta)sin\theta f'(\theta)sin\theta d\theta\n
=\frac12\int f(\theta)f'(\theta)(cos^2\theta-sin^2\theta)d\theta\n

\text{abandon du prof}
$$
